#+title: Claw Contraption

Part1 and part2 is solved analytically in the same way, except for the price
increase of part2.

The system of equations is as follows:

\begin{equation*}
\begin{cases}
a_{n} \cdot a_{x} + b_{n} \cdot b_{x} = p_{x} \\
a_{n} \cdot a_{y} + b_{n} \cdot b_{y} = p_{y}
\end{cases}
\end{equation*}

For the problem to make sense, we assume there is either 0 solutions or a single
solution to the problem.

To solve for $b_{n}$:

- Multiply the first equation by $a_{y}$ and the second by $a_{x}$ to eliminate $a_{n}$:
  $$
  (a_{n} \cdot a_{x} + b_{n} \cdot b_{x}) \cdot a_{y} = p_{x} \cdot a_{y}
  $$
  $$
  (a_{n} \cdot a_{y} + b_{n} \cdot b_{y}) \cdot a_{x} = p_{y} \cdot a_{x}
  $$

- Subtract the equations:
  $$
  b_{n} \cdot (b_{x} \cdot a_{y} - b_{y} \cdot a_{x}) = p_{x} \cdot a_{y} - p_{y} \cdot a_{x}
  $$

- Therefore, we solve for $b_{n}$:
  $$
  b_{n} = \frac{p_{x} \cdot a_{y} - p_{y} \cdot a_{x}}{b_{x} \cdot a_{y} - b_{y} \cdot a_{x}}
  $$

To solve for $a_{n}$:

- Substitute $b_{n}$ back into the first equation:
  $$
  a_{n} \cdot a_{x} + b_{n} \cdot b_{x} = p_{x}
  $$

  $$
  a_{n} \cdot a_{x} = p_{x} - b_{n} \cdot b_{x}
  $$

- Therefore, we solve for $a_{n}$:
  $$
  a_{n} = \frac{p_{x} - b_{n} \cdot b_{x}}{a_{x}}
  $$
